src/StackCompCombined.v
@@ -1,0 +1,115 @@
+Require Import compcert.driver.Compiler compcert.common.Errors.
+Require Import Common Monads.
+Require CompilationUnit.
+Require Import Metadata.
+
+Require ValueFlag StackFlatter2.
+Require
+    StackMachComp
+    StackContComp
+    StackContComp2
+    StackContComp3
+    StackFlatComp
+    StackFlatterComp
+    StackFlatterComp2
+.
+
+Definition option_to_res {A} (o : option A) : res A :=
+  match o with
+  | None => Error []
+  | Some a => OK a
+  end.
+Coercion option_to_res : option >-> res.
+
+Definition compile_cu (cu : ValueFlag.env * list metadata) :
+        res (StackFlatter2.env * list metadata) :=
+  OK cu
+  @@ StackMachComp.compile_cu
+  @@ StackContComp.compile_cu
+  @@ StackContComp2.compile_cu
+  @@ StackContComp3.compile_cu
+  @@ StackFlatComp.compile_cu
+  @@ StackFlatterComp.compile_cu
+  @@ StackFlatterComp2.compile_cu
+.
+
+Inductive I : ValueFlag.state -> StackFlatter2.state -> Prop :=
+| ICombined : forall s00 s01 s02 s03 s04 s05 s06 s07,
+        StackMachComp.I         s00 s01 ->
+        StackContComp.I         s01 s02 ->
+        StackContComp2.I        s02 s03 ->
+        StackContComp3.I        s03 s04 ->
+        StackFlatComp.I         s04 s05 ->
+        StackFlatterComp.I      s05 s06 ->
+        StackFlatterComp2.I     s06 s07 ->
+        I s00 s07.
+
+Inductive I_func : ValueFlag.expr -> list StackFlatter2.insn -> Prop :=
+| IFuncCombined : forall f00 f01 f02 f03 f04 f05 f06 f07,
+        StackMachComp.I_expr []             f00 f01 ->
+        Forall2 StackContComp.I_insn        f01 f02 ->
+        Forall2 StackContComp2.I_insn       f02 f03 ->
+        Forall2 StackContComp3.I_insn       f03 f04 ->
+        Forall2 StackFlatComp.I_insn        f04 f05 ->
+        StackFlatterComp.I_insns            f05 f06 ->
+        StackFlatterComp2.I_insns           f06 f07 ->
+        I_func f00 f07.
+
+
+Lemma chain_I_env :
+    forall e00 e01 e02 e03 e04 e05 e06 e07,
+        Forall2 (StackMachComp.I_expr [])           e00 e01 ->
+        Forall2 (Forall2 StackContComp.I_insn)      e01 e02 ->
+        Forall2 (Forall2 StackContComp2.I_insn)     e02 e03 ->
+        Forall2 (Forall2 StackContComp3.I_insn)     e03 e04 ->
+        Forall2 (Forall2 StackFlatComp.I_insn)      e04 e05 ->
+        Forall2 (StackFlatterComp.I_insns)          e05 e06 ->
+        Forall2 (StackFlatterComp2.I_insns)         e06 e07 ->
+        Forall2 I_func e00 e07.
+intros.
+list_magic_on (e00, (e01, (e02, (e03, (e04, (e05, (e06, (e07, tt)))))))).
+eapply IFuncCombined; eassumption.
+Qed.
+
+
+Ltac break_result_chain :=
+    let go l :=
+        match l with
+        | OK _ => fail 1
+        | _ => destruct l eqn:?; try discriminate
+        end in
+    repeat match goal with
+    | [ H : context [ ?l @@ ?r ] |- _ ] => go l
+    | [ H : context [ ?l @@@ ?r ] |- _ ] => go l
+    end.
+
+Ltac inject_ok :=
+    repeat match goal with
+    | [ H : OK ?x = OK ?y |- _ ] =>
+            assert (x = y) by congruence;
+            clear H
+    end.
+
+
+Theorem compile_I_func : forall a ameta b bmeta,
+    Forall ValueFlag.no_values a ->
+    compile_cu (a, ameta) = OK (b, bmeta) ->
+    Forall2 I_func a b.
+intros0 Hnval Hcomp. unfold compile_cu in *.
+
+remember (a, ameta) as aprog.
+break_result_chain.  simpl in *.  inject_ok.
+unfold option_to_res in *. repeat (break_match; try discriminate).
+subst aprog.  repeat on (_ * _)%type, fun x => destruct x.
+
+on _, eapply_lem StackMachComp.compile_cu_I_env; [ | auto ].
+on _, eapply_lem StackContComp.compile_cu_I_env.
+on _, eapply_lem StackContComp2.compile_cu_I_env.
+on _, eapply_lem StackContComp3.compile_cu_I_env.
+on _, eapply_lem StackFlatComp.compile_cu_I_env.
+on _, eapply_lem StackFlatterComp.compile_cu_I_env.
+on _, eapply_lem StackFlatterComp2.compile_cu_I_env.
+
+inject_ok. inject_pair.
+eapply chain_I_env; eassumption.
+Qed.
